more uniform flags for crypto games

examples/low-level/crypto/Crypto.Symmetric.Chacha20.PRF.fst
@@ -26,7 +26,7 @@ open Plain
 
 module HH = FStar.HyperHeap
 module HS = FStar.HyperStack
-
+  
 module MAC   = Crypto.Symmetric.Poly1305.MAC
 module Block = Crypto.Symmetric.BlockCipher
 
@@ -40,7 +40,8 @@ inline let authId (i: Plain.id) = Plain.authId i && Flag.prf i
 // second step: constrain use of PRF for authenticated encryption and decryption
 inline let safeId (i: Plain.id) = Plain.authId i && Flag.prf_enc i
 
-let _ = assert(forall i. safeId ==> authId)
+let sanity_check = assert(forall i. safeId i ==> authId i)
+
 
 // LIBRARY STUFF
 
@@ -86,12 +87,12 @@ noeq type otp i = | OTP: l:u32 {l <=^ blocklen} -> plain i (v l) -> cipher:lbyte
 let range (rgn:region) (i:id) (x:domain): Type0 =
   if x.ctr = 0ul then smac rgn i x
   else if safeId i then otp i
-  else lbytes blocklen
+  else lbytes (v blocklen)
 
 // explicit coercions
-let macRange rgn i (x:domain{x.ctr = 0ul}) (v:range rgn i x) : smac rgn i x = v
-let otpRange rgn i (x:domain{safeID i /\ x.ctr <> 0ul}) (v:range rgn i x) : otp i = v
-let blkRange rgn i (x:domain{~ (safeID) i /\ x.ctr <> 0ul}) (v:range rgn i x) : otp i = v
+let macRange rgn i (x:domain{x.ctr = 0ul}) (z:range rgn i x) : smac rgn i x = z
+let otpRange rgn i (x:domain{x.ctr <> 0ul /\ safeId i}) (z:range rgn i x) : otp i = z 
+let blkRange rgn i (x:domain{x.ctr <> 0ul /\ ~ (safeId i)}) (z:range rgn i x) : lbytes (v blocklen) = z
 
 noeq type entry (rgn:region) (i:id) =
   | Entry: x:domain -> range:range rgn i x -> entry rgn i
@@ -101,55 +102,66 @@ let find (#rgn:region) (#i:id) (s:Seq.seq (entry rgn i)) (x:domain) : option (ra
   | Some e -> Some e.range
   | None   -> None
 
-let find_0 #rgn #i s (x:domain{x.ctr=0ul}) =
+let find_mac #rgn #i s (x:domain{x.ctr=0ul}) =
   match find s x with
   | Some v -> Some(macRange rgn i x v)
   | None   -> None
 
-let find_1 #rgn #i s (x:domain{x.ctr<>0ul}) =
+let find_otp #rgn #i s (x:domain{x.ctr<>0ul /\ safeId i}) =
   match find s x with
   | Some v -> Some(otpRange rgn i x v)
   | None   -> None
 
+let find_blk #rgn #i s (x:domain{x.ctr<>0ul /\ ~(safeId i)}) =
+  match find s x with
+  | Some v -> Some (blkRange rgn i x v)
+  | None   -> None
+
+// The table exists only for idealization
+// TODO it should be a monotonic map: what's in the table stays there. 
+let table_t rgn i = 
+  if authId i then (r: HS.ref (Seq.seq (entry rgn i)) {HS.frameOf r = rgn})
+  else unit
+
 // the PRF instance, including its key and memoization table
 // TODO separate on rw, with multiple readers?
 noeq type state (i:id) =
-  | State: #rgn: region ->
-           // key is immutable once generated, we should rather use lbytes ...
-           key:lbuffer (v (Block.keylen prfa)) {Buffer.frameOf key = rgn} ->
-           (* TODO:
-           table:(
-             if Flag.prf i then
-               HS.ref (Seq.seq (entry rgn i)) {HS.frameOf table = rgn}
-             else
-               unit
-           ) -> *)
-           table:HS.ref (Seq.seq (entry rgn i)) {HS.frameOf table = rgn} ->
-           state i  // should be maybe_mrref; for later.
-// TODO the table should exist only when ideal, and should actually be a map.
-// TODO coerce, leak, and eventually dynamic compromise.
+  | State: #rgn: region -> 
+           // key is immutable once generated, we should make it private
+           key: lbuffer (v (Block.keylen prfa)) {Buffer.frameOf key = rgn} ->
+           table: table_t rgn i ->
+           state i
+
+// boring...
+val itable: i:id {authId i} -> s:state i  -> Tot (r: HS.ref (Seq.seq (entry s.rgn i)) {HS.frameOf r = s.rgn})
+let itable i s = s.table
+val mktable: i:id {authId i} -> rgn:region -> r: HS.ref (Seq.seq (entry rgn i)) {HS.frameOf r = rgn} -> Tot (table_t rgn i)
+let mktable i rgn r = r 
+val no_table: i:id {~(authId i)} -> rgn:region -> Tot (table_t rgn i)
+let no_table i rgn = ()
+
 
 val gen: rgn:region -> i:id -> ST (state i)
   (requires (fun h -> True))
   (ensures  (fun h0 s h1 ->
-    s.rgn == rgn /\ HS.sel h1 s.table == Seq.createEmpty #(entry rgn i)))
+    s.rgn == rgn /\ 
+    (authId i ==> HS.sel h1 (itable i s) == Seq.createEmpty #(entry rgn i))))
 let gen rgn i =
-  // SZ: let key = MAC.random rgn Block.keylen`?
   let key = Buffer.rcreate rgn 0uy (Block.keylen prfa) in
   store_bytes (Block.keylen prfa) key (random (Block.keylen prfa));
-  let table = ralloc rgn (Seq.createEmpty #(entry rgn i)) in
+  let table = if authId i then mktable i rgn (ralloc rgn (Seq.createEmpty #(entry rgn i))) else () in
   State #i #rgn key table
-
+// no need to demand authId i so far.
 
 val coerce: rgn:region -> i:id{~(authId i)} -> key:lbuffer (v keylen) -> ST (state i)
   (requires (fun h -> Buffer.live h key))
-  (ensures  (fun h0 s h1 ->
-    s.rgn == rgn /\ HS.sel h1 s.table == Seq.createEmpty #(entry rgn i)))
+  (ensures  (fun h0 s h1 -> s.rgn == rgn))
 let coerce rgn i key =
   let key_p = Buffer.rcreate rgn 0uy (Block.keylen prfa) in
   Buffer.blit key 0ul key_p 0ul (Block.keylen prfa);
-  let table = ralloc rgn (Seq.createEmpty #(entry rgn i)) in // Shoudln't exist
-  State #i #rgn key_p table
+  State #i #rgn key_p (no_table i rgn)
+
+// TODO leak, and eventually dynamic compromise.
 
 
 (** computes a PRF block and copies its len first bytes to output *)
@@ -180,12 +192,58 @@ val prf_mac: i:id -> t:state i -> x:domain{x.ctr = 0ul} -> ST (MAC.state (i,x.iv
   (requires (fun h0 -> True))
   (ensures (fun h0 mac h1 ->
     authId i ==>
-    ( match find_0 (HS.sel h1 t.table) x with
+    ( match find_mac (HS.sel h1 (itable i t)) x with
       | Some mac' -> mac == mac' /\ MAC.genPost (i,x.iv) t.rgn h0 mac h1
       | None      -> False
     // we guarantee the stateful post of MAC.create when x is not in the table.
     // in all cases, we return the state in the table
   )))
+
+// real case + real use of memoized PRF output.
+private val prf_raw: 
+  i:id -> t:state i -> x:domain{~(safeId i) /\ x.ctr <> 0ul} ->
+  l:u32 {l <=^ blocklen} -> output:lbuffer (v l) -> ST unit
+  (requires (fun h0 -> Buffer.live h0 output))
+  (ensures (fun h0 _ h1 -> 
+    Buffer.live h1 output /\ 
+    if authId i then (
+      // 16-10-08 this is gross; we need nicer libraries!
+      // I just want to write modifies !{ itable i t, output } h0 h1
+      // we should never have to refer to several of H, HH, HS, HST (and maybe Buffer) at the same time!
+      // can't get any concrete syntax for sets to work below.
+      let r = itable i t in 
+      let rb = Buffer.frameOf output in 
+      // can't use !{ t.rgn, rb}, why?
+      let rgns = Set.union (Set.singleton #HH.rid t.rgn) (Set.singleton #HH.rid rb) in 
+      Buffer.live h1 output /\ 
+      HS.modifies rgns h0 h1 /\ 
+      HS.modifies_ref t.rgn (TSet.singleton (FStar.Heap.Ref (HS.as_ref r))) h0 h1 /\
+      Buffer.modifies_bufs rb (TSet.singleton (Buffer.Buff output)) h0 h1 )
+    else
+      Buffer.modifies_1 output h0 h1
+    ))
+
+let prf_raw i t x l output = 
+  if authId i then (
+    recall (itable i t);
+    let table = !(itable i t) in
+    let block = 
+      ( match find_blk table x with 
+      | Some block -> block 
+      | None -> (
+          let block = random blocklen in 
+          t.table := SeqProperties.snoc table (Entry x block);
+          let h = HST.get() in 
+          assert(Buffer.live h output);
+          block )) in
+    //assume false;
+    let h = HST.get() in 
+    assert(Buffer.live h output);
+    store_bytes l output (Seq.slice block 0 (v l)))
+  else 
+    getBlock t x l output 
+
+
 
 // reuse the same block for x and XORs it with ciphertext
 val prf_dexor: i:id -> t:state i -> x:domain{x.ctr <> 0ul} ->
@@ -194,7 +252,7 @@ val prf_dexor: i:id -> t:state i -> x:domain{x.ctr <> 0ul} ->
      Plain.live h0 plain /\ Buffer.live h0 cipher /\ Buffer.disjoint (bufferT plain) cipher /\
      Buffer.frameOf (bufferT plain) <> t.rgn /\
      (safeId i ==>
-     ( match find_1 (HS.sel h0 t.table) x with
+     ( match find_otp (HS.sel h0 t.table) x with
        | Some (OTP l' p c) -> l == l' /\ c == sel_bytes h0 l cipher
        | None -> False
      ))))
@@ -202,31 +260,31 @@ val prf_dexor: i:id -> t:state i -> x:domain{x.ctr <> 0ul} ->
      Plain.live h1 plain /\ Buffer.live h1 cipher /\
      Buffer.modifies_1 (bufferT plain) h0 h1 /\
      (safeId i ==>
-       ( match find_1 (HS.sel h1 t.table) x with
+       ( match find_otp (HS.sel h1 t.table) x with
          | Some (OTP l' p c) -> l == l' /\ p == sel_plain h1 l plain
          | None -> False
      ))))
 
 let prf_dexor i t x l plain cipher =
-  if authId i then
+  if safeId i then
     begin
       recall t.table;
       let contents = !t.table in
-      match find_1 contents x with
-      | Some (OTP l' p c) -> (
-          let h0 = HST.get() in
-          Plain.store #i l plain p;
-          let h1 = HST.get() in
-          Buffer.lemma_reveal_modifies_1 (bufferT plain) h0 h1)
+        match find_otp contents x with
+        | Some (OTP l' p c) -> (
+            let h0 = HST.get() in
+            Plain.store #i l plain p;
+            let h1 = HST.get() in
+            Buffer.lemma_reveal_modifies_1 (bufferT plain) h0 h1)
 //          let contents' = !t.table in
 //          assert(Buffer.frameOf (bufferT plain) <> t.rgn);
 //          assert(contents == contents')
     end
   else
     begin
-      let plain = bufferRepr #i #(v l) plain in
-      getBlock t x l plain;
-      Buffer.Utils.xor_bytes_inplace plain cipher l
+      let plainrepr = bufferRepr #i #(v l) plain in
+      prf_raw i t x l plainrepr; 
+      Buffer.Utils.xor_bytes_inplace plainrepr cipher l
     end
 
 //TODO (NS): this one takes about 15s to prove automatically; investigate a bit
@@ -245,18 +303,18 @@ val prf_enxor: i:id -> t:state i -> x:domain{x.ctr <> 0ul} ->
      Buffer.frameOf cipher <> t.rgn /\
      Plain.live h0 plain /\ Buffer.live h0 cipher /\
      Buffer.disjoint (bufferT plain) cipher /\
-     is_None(find_1 (HS.sel h0 t.table) x)
+     is_None(find_otp (HS.sel h0 t.table) x)
      ))
   (ensures (fun h0 _ h1 ->
      Plain.live h1 plain /\ Buffer.live h1 cipher /\
      Buffer.modifies_1 cipher h0 h1 /\ //16-09-22 missing hybrid modifies also covering t.
      (authId i ==>
-       ( match find_1 (HS.sel h1 t.table) x with
+       ( match find_otp (HS.sel h1 t.table) x with
          | Some (OTP l' p c) -> l = l' /\ p == sel_plain h1 l plain /\ c == sel_bytes h1 l cipher
          | None   -> False
      ))))
 let prf_enxor i t x l cipher plain =
-  if authId i then
+  if safeId i then
     begin
       recall t.table;
       let p = Plain.load #i l plain in
@@ -265,14 +323,14 @@ let prf_enxor i t x l cipher plain =
       assume false;//16-10-02
       let contents = !t.table in //NS: Or, we can move this read up; but the anti-aliasing seems like the right thing to do
       let newblock = OTP #i l p c in
-      assert(find contents x == None); //TODO how to avoid explicit annotations on find_1 ? NS: find_1 is fine here; without the store_bytes this assertion succeeds
+      assert(find contents x == None); //TODO how to avoid explicit annotations on find_otp ? NS: find_otp is fine here; without the store_bytes this assertion succeeds
       lemma_snoc_found contents x newblock;
       t.table := SeqProperties.snoc contents (Entry x newblock) //NS: t.table is mutated;  so the modifies_1 cipher h0 h1 cannot be true
     end
   else
     begin
-      let plain = bufferRepr #i #(v l) plain in
-      getBlock t x l cipher;
+      let plainrepr = bufferRepr #i #(v l) plain in
+      prf_raw i t x l cipher;
       Buffer.Utils.xor_bytes_inplace cipher plain l
     end
 
@@ -282,7 +340,7 @@ let prf_mac i t x =
       assume false; //16-10-02
       recall t.table;
       let contents = !t.table in //TODO unclear which pre is missing
-      match find_0 contents x with
+      match find_mac contents x with
       | Some mac -> mac
       | None     ->
         begin
