examples/low-level/crypto/Flag.fsti
@@ -1,43 +1,96 @@
 module Flag
 
-open Crypto.Symmetric
+(* floating *) 
 
-(** All the idealization flags that we use for the cryptographic argument *)
+type mac_alg =
+  | POLY1305
+  | GHASH
 
-val aes_prf:bool
-val chacha20_prf:bool
+type aead_cipher =
+  | AES_256_GCM
+  | CHACHA20_POLY1305
 
-// TODO check with Nik that this will normalize properly when all branches
-// evaluate to false
-let prf (i: Plain.id) =
-  match BlockCipher.alg_of_id i with
-  | BlockCipher.AES256 -> aes_prf
-  | BlockCipher.CHACHA20 -> chacha20_prf
+type id = {
+  cipher: aead_cipher;
+  uniq: UInt32.t // we'll need more
+}
 
-val poly1305_mac1: bool
-val ghash_mac1: bool
+inline let mac_of_id i =
+  match i.cipher with
+  | AES_256_GCM       -> GHASH
+  | CHACHA20_POLY1305 -> POLY1305
 
-val mac_log: bool
+inline let cipher_of_id i =
+  let open Crypto.Symmetric.BlockCipher in 
+  match i.cipher with
+  | AES_256_GCM       -> AES256
+  | CHACHA20_POLY1305 -> CHACHA20
 
-let mac1 (i: Plain.id) =
-  let open Plain in
-  match mac_alg_of_id i with
-  | POLY1305 -> poly1305_mac1 && mac_log
-  | GHASH -> ghash_mac1 && mac_log
+inline let cipher_alg = Crypto.Symmetric.BlockCipher.alg
 
-val mac1_implies_mac_log: i:Plain.id -> Lemma
-  (requires True)
-  (ensures (mac1 i ==> mac_log))
+(* All the idealization flags that we use for the cryptographic argument *)
+
+// TODO check that the real implementation normalizes fully.
+
+
+(* CRYPTOGRAPHIC SECURITY ASSUMPTIONS.
+   These are not conditioned by i. 
+   They suffice to select every intermediate game in our proof.
+   They are ordered as successive idealization steps in our proof.
+   We used to refer to those as "algorithmic strength predicates".
+*) 
+
+// controls idealization of each cipher as a perfect random function
+val cipher_prf: cipher_alg -> Tot bool 
+
+// controls existence of logs for all MACs
+val mac_log: bool                
+
+// idealizes each one-time MAC as perfectly INT-1CMA.
+val mac_int1cma: mac_alg -> Tot bool  
+
+// controls 2nd, perfect idealization step in enxor/dexor for all PRFs.
+val prf_cpa: bool
+
+
+(* CONDITIONAL IDEALIZATION *) 
+
+// guarantees fresh record keys (to be defined by TLS Handshake)
+val safeHS: i:id -> Tot bool 
+
+// controls PRF idealization of ciphers (move to PRF?)
+inline let prf (i: id) = safeHS i && cipher_prf(cipher_of_id i)
+
+// controls INT1CMA idealization of MACs (move to MAC?)
+inline let mac1 i = mac_log && mac_int1cma (mac_of_id i)
+
+// controls abstraction of plaintexts
+// (kept abstract, but requires all the crypto steps above)
+val safeId: i:id -> Tot bool
+
+
+(* IDEALIZATION DEPENDENCIES *) 
+
+// review usage of these lemmas
+
+val mac1_implies_mac_log: i:id -> Lemma
+  (requires (mac1 i))
+  (ensures mac_log)
   [SMTPat (mac1 i)]
 
-val mac1_implies_prf: i:Plain.id -> Lemma
-  (requires True)
-  (ensures (mac1 i ==> prf i))
+val mac1_implies_prf: i:id -> Lemma
+  (requires (mac1 i))
+  (ensures (prf i))
   [SMTPat (mac1 i)]
 
-val prf_enc: i:Plain.id -> Tot bool
+val safeId_implies_mac1: i:id -> Lemma
+  (requires (safeId i))
+  (ensures (mac1 i))
+  [SMTPat (safeId i)]
 
-val prf_enc_implies_mac1: i:Plain.id -> Lemma
-  (requires True)
-  (ensures (prf_enc i ==> mac1 i))
-  [SMTPat (prf_enc i)]
+val safeId_implies_cpa: i:id -> Lemma
+  (requires (safeId i))
+  (ensures (prf_cpa))
+  [SMTPat (safeId i)]
+
+
