examples/low-level/crypto/Crypto.Symmetric.BlockCipher.fst
@@ -18,12 +18,6 @@ type alg =
   | AES256
   | CHACHA20 // RFC 7539 for the AEAD algorithm; RFC 7905 for the TLS ciphersuites
 
-let alg_of_id (id: Plain.id): alg =
-  let open Plain in
-  match id.cipher with
-  | AES_256_GCM -> AES256
-  | CHACHA20_POLY1305 -> CHACHA20
-
 let keylen = function
 //| AES128   -> 16ul
   | AES256   -> 32ul
